src/backend/dafny/Havoc.dfy
@@ -1,0 +1,114 @@
+include "Lang.dfy"
+include "Print.dfy"
+
+function method digitToString(n: nat): string
+  requires 0 <= n <= 9
+{
+  var digits := ["0", "1", "2", "3", "4", "5", "6", "7", "8", "9"];
+  digits[n]
+}
+
+
+function method natToString(n: nat): string
+{
+  if (n <= 9) then digitToString(n)
+  else natToString(n/10) + digitToString(n % 10)
+}
+
+
+class Havocer
+{
+  var nextId: nat;
+  var newVars: seq<(nat, string)>;
+
+  const havocPrefix: string;
+
+  constructor(havocPrefix: string)
+  {
+    nextId := 0;
+    // TODO: make sure to avoid clashes with existing variables by setting this to something unused
+    // by concrete programs.
+    this.havocPrefix := havocPrefix;
+  }
+
+  method freshId(rhs: string) returns (id: nat)
+    modifies this
+  {
+    id := nextId;
+    newVars := newVars + [(id, rhs)];
+    nextId := nextId + 1;
+  }
+
+  function method varName(n: nat): string
+  {
+    havocPrefix + natToString(n)
+  }
+
+  // AssocGet(AssocGet(objs, addr).val.locals, "x")
+  method havocLocals(locals: List<Pair<Var, Value>>, immuts: List<Var>, addr: Addr)
+    returns (newLocals: List<Pair<Var, Value>>)
+    modifies this
+    decreases locals
+  {
+    match locals {
+      case LNil => { newLocals := LNil(); }
+      case Cons(Pair(name, val), locals') => {
+        var rest := havocLocals(locals', immuts, addr);
+        if InList(immuts, name) {
+          newLocals := Cons(Pair(name, val), rest);
+
+        } else {
+          var next := freshId("AssocGet(AssocGet({objs}, " + natToString(addr) + ").val.locals, \\\"" + name + "\\\").val");
+          newLocals := Cons(Pair(name, Internal(varName(next))), rest);
+        }
+      }
+    }
+  }
+
+  method havocObj(obj: Object, addr: Addr) returns (newObj: Object)
+    modifies this
+  {
+    var newLocals := havocLocals(obj.locals, obj.immutables, addr);
+    newObj := obj.(locals := newLocals);
+  }
+
+  method havocObjs(objs: ObjList) returns (newObjs: ObjList)
+    modifies this
+  {
+    match objs {
+      case LNil => { newObjs := LNil(); }
+      case Cons(Pair(addr, obj), objs') => {
+        var newObj := havocObj(obj, addr);
+        var rest := havocObjs(objs');
+        newObjs := Cons(Pair(addr, newObj), rest);
+      }
+    }
+  }
+
+  method VarsToString(vars: seq<(nat, string)>) returns (varNames: seq<string>)
+  {
+    if vars == [] {
+      varNames := [];
+    } else {
+      var i: int := |vars| - 1;
+      varNames := [];
+      while i >= 0
+      invariant -1 <= i < |vars|
+      decreases i
+      {
+        var (varId, varVal) := vars[i];
+        varNames := ["(\"" + varName(varId) + "\", \"" + varVal + "\")"] + varNames;
+        i := i - 1;
+      }
+    }
+  }
+
+  method printHavocData(stuff: (Value, Context))
+    modifies this
+  {
+    var objs := havocObjs(stuff.1.objs);
+    // TODO: use a proper output format here in case this optimization turns out to be useful
+    var newVarNames := VarsToString(newVars);
+    print quoteObjs(objs), " @@@ ", newVarNames;
+  }
+}
