src/backend/dafny/Util.dfy
@@ -1,0 +1,1 @@
+const True := true; const False := false;
